theories/datatypes_properties.v
@@ -287,3 +287,12 @@ Definition eqtable_typeP : Equality.axiom table_type_eqb :=
 
 Canonical Structure table_type_eqMixin := EqMixin eqtable_typeP.
 Canonical Structure table_type_eqType := Eval hnf in EqType table_type table_type_eqMixin.
+
+Definition mem_type_eq_dec : forall v1 v2 : mem_type, {v1 = v2} + {v1 <> v2}.
+Proof. decidable_equality. Defined.
+Definition mem_type_eqb v1 v2 : bool := mem_type_eq_dec v1 v2.
+Definition eqmem_typeP : Equality.axiom mem_type_eqb :=
+  eq_dec_Equality_axiom mem_type_eq_dec.
+
+Canonical Structure mem_type_eqMixin := EqMixin eqmem_typeP.
+Canonical Structure mem_type_eqType := Eval hnf in EqType mem_type mem_type_eqMixin.
