theories/instantiation.v
@@ -1,5 +1,6 @@
 From mathcomp Require Import ssreflect ssrbool ssrnat eqtype seq.
 Require Import datatypes datatypes_properties.
+Require interpreter.
 Require binary_format_parser operations typing opsem.
 (* TODO: separate algorithmic aspects from specification, incl. dependencies *)
 
@@ -11,7 +12,7 @@ Definition tableaddr := addr.
 Definition memaddr := addr.
 Definition globaladdr := addr.
 
-Definition alloc_Xs {A} f (s : store_record) (xs : list A) : store_record * list nat :=
+Definition alloc_Xs {A B} f (s : store_record) (xs : list A) : store_record * list B :=
   let '(s', fas) :=
     List.fold_left
       (fun '(s, ys) x =>
@@ -46,14 +47,14 @@ Definition add_func (s : store_record) funcinst := {|
   s_globals := s.(s_globals);
 |}.
 
-Definition alloc_func (s : store_record) (m_f : module_func) (mi : instance) : store_record * nat :=
+Definition alloc_func (s : store_record) (m_f : module_func) (mi : instance) : store_record * funcidx :=
   let funcaddr := List.length s.(s_funcs) in
   let functype := List.nth (match m_f.(mf_type) with | Mk_typeidx n => n end) mi.(i_types) (Tf nil nil (* TODO: partiality problem *) ) in
   let funcinst := Func_native mi functype m_f.(mf_locals) m_f.(mf_body) in
   let S' := add_func s funcinst in
-  (S', funcaddr).
+  (S', Mk_funcidx funcaddr).
 
-Definition alloc_funcs (s : store_record) (m_fs : list module_func) (mi : instance) : store_record * list nat :=
+Definition alloc_funcs (s : store_record) (m_fs : list module_func) (mi : instance) : store_record * list funcidx :=
   alloc_Xs (fun s m_f => alloc_func s m_f mi) s m_fs.
 
 Definition add_table (s : store_record) (ti : tableinst) : store_record := {|
@@ -63,13 +64,13 @@ Definition add_table (s : store_record) (ti : tableinst) : store_record := {|
   s_globals := s.(s_globals);
 |}.
 
-Definition alloc_tab (s : store_record) (tty : table_type) : store_record * nat :=
+Definition alloc_tab (s : store_record) (tty : table_type) : store_record * tableidx :=
   let '{| tt_limits := {| lim_min := min; lim_max := maxo |} as lim; tt_elem_type := ety |} := tty in
-  let tableaddr := List.length s.(s_tables) in
+  let tableaddr := Mk_tableidx (List.length s.(s_tables)) in
   let tableinst := {| table_data := (List.repeat None min); table_max_opt := maxo; |} in
   (add_table s tableinst, tableaddr).
 
-Definition alloc_tabs (s : store_record) (ts : list table_type) : store_record * list nat :=
+Definition alloc_tabs (s : store_record) (ts : list table_type) : store_record * list tableidx :=
   alloc_Xs alloc_tab s ts.
 
 Definition ki64 : nat := 65536.
@@ -84,13 +85,14 @@ Definition add_mem (s : store_record) (m_m : memory) : store_record := {|
   s_globals := s.(s_globals);
 |}.
 
-Definition alloc_mem (s : store_record) (m_m : mem_type) : store_record * nat :=
-  let '{| lim_min := min; lim_max := maxo |} := m_m in
-  let memaddr := List.length s.(s_mems) in
-  let meminst := mem_mk m_m in
+Definition alloc_mem (s : store_record) (m_m : mem_type) : store_record * memidx :=
+  let 'Mk_mem_type lims := m_m in
+  let '{| lim_min := min; lim_max := maxo |} := lims in
+  let memaddr := Mk_memidx (List.length s.(s_mems)) in
+  let meminst := mem_mk lims in
   (add_mem s meminst, memaddr).
 
-Definition alloc_mems (s : store_record) (m_ms : list mem_type) : store_record * list nat :=
+Definition alloc_mems (s : store_record) (m_ms : list mem_type) : store_record * list memidx :=
   alloc_Xs alloc_mem s m_ms.
 
 Definition add_glob (s : store_record) (m_g : global) : store_record := {|
@@ -100,9 +102,9 @@ Definition add_glob (s : store_record) (m_g : global) : store_record := {|
   s_globals := List.app s.(s_globals) (cons m_g nil);
 |}.
 
-Definition alloc_glob (s : store_record) (m_g_v : module_glob * value) : store_record * nat :=
+Definition alloc_glob (s : store_record) (m_g_v : module_glob * value) : store_record * globalidx :=
   let '(m_g, v) := m_g_v in
-  let globaddr := List.length s.(s_globals) in
+  let globaddr := Mk_globalidx (List.length s.(s_globals)) in
   let globinst := Build_global m_g.(mg_type).(tg_mut) v in
   (add_glob s globinst, globaddr).
 
@@ -116,10 +118,10 @@ Definition v_ext := module_export_desc.
 Definition export_get_v_ext (inst : instance) (exp : module_export_desc) : v_ext :=
   (* we circumvent partiality by providing 0 as a default *)
   match exp with
-  | ED_func i => ED_func (List.nth i inst.(i_funcs) 0)
-  | ED_table i => ED_table (List.nth i inst.(i_tab) 0)
-  | ED_mem i => ED_mem (List.nth i inst.(i_memory) 0)
-  | ED_global i => ED_global (List.nth i inst.(i_globs) 0)
+  | ED_func (Mk_funcidx i) => ED_func (Mk_funcidx (List.nth i inst.(i_funcs) 0))
+  | ED_table (Mk_tableidx i) => ED_table (Mk_tableidx (List.nth i inst.(i_tab) 0))
+  | ED_mem (Mk_memidx i) => ED_mem (Mk_memidx (List.nth i inst.(i_memory) 0))
+  | ED_global (Mk_globalidx i) => ED_global (Mk_globalidx (List.nth i inst.(i_globs) 0))
   end.
 
 Definition ext_funcs :=
@@ -193,23 +195,23 @@ Definition alloc_module (s : store_record) (m : module) (imps : list v_ext) (gvs
   let '(s3, i_ms) := alloc_mems s2 m.(mod_mems) in
   let '(s', i_gs) := alloc_globs s3 m.(mod_globals) gvs in
   (inst.(i_types) == m.(mod_types)) &&
-  (inst.(i_funcs) == List.app (ext_funcs imps) i_fs) &&
-  (inst.(i_tab) == List.app (ext_tabs imps) i_ts) &&
-  (inst.(i_memory) == List.app (ext_mems imps) i_ms) &&
-  (inst.(i_globs) == List.app (ext_globs imps) i_gs) &&
+  (inst.(i_funcs) == List.map (fun '(Mk_funcidx i) => i) (List.app (ext_funcs imps) i_fs)) &&
+  (inst.(i_tab) == List.map (fun '(Mk_tableidx i) => i) (List.app (ext_tabs imps) i_ts)) &&
+  (inst.(i_memory) == List.map (fun '(Mk_memidx i) => i) (List.app (ext_mems imps) i_ms)) &&
+  (inst.(i_globs) == List.map (fun '(Mk_globalidx i) => i) (List.app (ext_globs imps) i_gs)) &&
   (exps == List.map (fun m_exp => {| exp_name := m_exp.(exp_name); exp_desc := (export_get_v_ext inst m_exp.(exp_desc)) |}) m.(mod_exports)).
 
 Definition interp_alloc_module (s : store_record) (m : module) (imps : list v_ext) (gvs : list value) : (store_record * instance * list module_export) :=
-  let i_fs := seq.iota (List.length s.(s_funcs)) (List.length m.(mod_funcs)) in
-  let i_ts := seq.iota (List.length s.(s_tables)) (List.length m.(mod_tables)) in
-  let i_ms := seq.iota (List.length s.(s_mems)) (List.length m.(mod_mems)) in
-  let i_gs := seq.iota (List.length s.(s_globals)) (min (List.length m.(mod_globals)) (List.length gvs)) in
+  let i_fs := List.map (fun i => Mk_funcidx i) (seq.iota (List.length s.(s_funcs)) (List.length m.(mod_funcs))) in
+  let i_ts := List.map (fun i => Mk_tableidx i) (seq.iota (List.length s.(s_tables)) (List.length m.(mod_tables))) in
+  let i_ms := List.map (fun i => Mk_memidx i) (seq.iota (List.length s.(s_mems)) (List.length m.(mod_mems))) in
+  let i_gs := List.map (fun i => Mk_globalidx i) (seq.iota (List.length s.(s_globals)) (min (List.length m.(mod_globals)) (List.length gvs))) in
   let inst := {|
     i_types := m.(mod_types);
-    i_funcs := List.app (ext_funcs imps) i_fs;
-    i_tab := List.app (ext_tabs imps) i_ts;
-    i_memory := List.app (ext_mems imps) i_ms;
-    i_globs := List.app (ext_globs imps) i_gs;
+    i_funcs := List.map (fun '(Mk_funcidx i) => i) (List.app (ext_funcs imps) i_fs);
+    i_tab := List.map (fun '(Mk_tableidx i) => i) (List.app (ext_tabs imps) i_ts);
+    i_memory := List.map (fun '(Mk_memidx i) => i) (List.app (ext_mems imps) i_ms);
+    i_globs := List.map (fun '(Mk_globalidx i) => i) (List.app (ext_globs imps) i_gs);
   |} in
   let '(s1, _) := alloc_funcs s m.(mod_funcs) inst in
   let '(s2, _) := alloc_tabs s1 (List.map (fun t => t.(t_type)) m.(mod_tables)) in
@@ -226,9 +228,9 @@ List.app (List.firstn n l) (List.app (cons v nil) (List.skipn (n + 1) l)).
 Definition dummy_table := {| table_data := nil; table_max_opt := None; |}.
 
 Definition init_tab (s : store_record) (inst : instance) (e_ind : nat) (e : module_element) : store_record :=
-  let t_ind := List.nth e.(elem_table) inst.(i_tab) 0 in
+  let t_ind := List.nth (match e.(elem_table) with Mk_tableidx i => i end) inst.(i_tab) 0 in
   let '{|table_data := tab_e; table_max_opt := maxo |} := List.nth t_ind s.(s_tables) dummy_table in
-  let e_pay := List.map (fun i => List.nth_error inst.(i_funcs) i) e.(elem_init) in
+  let e_pay := List.map (fun i => List.nth_error inst.(i_funcs) (match i with Mk_funcidx j => j end)) e.(elem_init) in
   let tab'_e := List.app (List.firstn e_ind tab_e) (List.app e_pay (List.skipn (e_ind + length e_pay) tab_e)) in
   {| s_funcs := s.(s_funcs);
      s_tables := insert_at {| table_data := tab'_e; table_max_opt := maxo |} e_ind s.(s_tables);
@@ -241,7 +243,7 @@ Definition init_tabs (s : store_record) (inst : instance) (e_inds : list nat) (e
 Definition dummy_mem := {| mem_data := nil; mem_limit := {| lim_min := 0; lim_max := None; |} |}.
 
 Definition init_mem (s : store_record) (inst : instance) (d_ind : nat) (d : module_data) : store_record :=
-  let m_ind := List.nth d.(dt_data) inst.(i_memory) 0 in
+  let m_ind := List.nth (match d.(dt_data) with Mk_memidx i => i end) inst.(i_memory) 0 in
   let mem := List.nth m_ind s.(s_mems) dummy_mem in
   let mem' := operations.write_bytes mem d_ind (List.map compcert_byte_of_byte d.(dt_init)) in
   {| s_funcs := s.(s_funcs);
@@ -279,7 +281,8 @@ Definition module_tab_typing (t : module_table) : bool :=
   limit_typing t.(t_type).(tt_limits) (expn_rec 2 32).
 
 Definition module_mem_typing (m : mem_type) : bool :=
-  limit_typing m (expn_rec 2 32).
+  let '(Mk_mem_type lim) := m in
+  limit_typing lim (expn_rec 2 32).
 
 Definition const_expr (c : t_context) (b_e : basic_instruction) : bool :=
   match b_e with
@@ -302,20 +305,20 @@ Definition module_glob_typing (c : t_context) (g : module_glob) (tg : global_typ
   typing.be_typing c es (Tf nil (cons tg.(tg_t) nil)).
 
 Definition module_elem_typing (c : t_context) (e : module_element) : Prop :=
-  let '{| elem_table := t; elem_offset := es; elem_init := is_ |} := e in
+  let '{| elem_table := Mk_tableidx t; elem_offset := es; elem_init := is_ |} := e in
   const_exprs c es /\
   typing.be_typing c es (Tf nil (cons T_i32 nil)) /\
   t < List.length c.(tc_table) /\
-  seq.all (fun i => i < List.length c.(tc_func_t)) is_.
+  seq.all (fun '(Mk_funcidx i) => i < List.length c.(tc_func_t)) is_.
 
 Definition module_data_typing (c : t_context) (m_d : module_data) : Prop :=
-  let '{| dt_data := d; dt_offset := es; dt_init := bs |} := m_d in
+  let '{| dt_data := Mk_memidx d; dt_offset := es; dt_init := bs |} := m_d in
   const_exprs c es /\
   typing.be_typing c es (Tf nil (cons T_i32 nil)) /\
   d < List.length c.(tc_memory).
 
 Definition module_start_typing (c : t_context) (ms : module_start) : bool :=
-  let i := ms.(start_func) in
+  let '(Mk_funcidx i) := ms.(start_func) in
   (i < length c.(tc_func_t)) &&
   match List.nth_error c.(tc_func_t) i with
   | None => false
@@ -340,25 +343,25 @@ Definition module_import_typing (c : t_context) (d : import_desc) (e : extern_t)
 
 Definition module_export_typing (c : t_context) (d : module_export_desc) (e : extern_t) : bool :=
   match (d, e) with
-  | (ED_func i, ET_func tf) =>
+  | (ED_func (Mk_funcidx i), ET_func tf) =>
     (i < List.length c.(tc_func_t)) &&
     match List.nth_error c.(tc_func_t) i with
     | None => false
     | Some tf' => tf == tf'
     end
-  | (ED_table i, ET_tab t_t) =>
+  | (ED_table (Mk_tableidx i), ET_tab t_t) =>
     (i < List.length c.(tc_table)) &&
     match List.nth_error c.(tc_table) i with
     | None => false
     | Some t_t' => t_t == t_t'
     end
-  | (ED_mem i, ET_mem mt) =>
+  | (ED_mem (Mk_memidx i), ET_mem (Mk_mem_type lim)) =>
     (i < List.length c.(tc_memory)) &&
     match List.nth_error c.(tc_memory) i with
     | None => false
-    | Some mt' => mt == mt'
+    | Some lim' => lim == lim' (* TODO: should check for equality of `mem_type`s *)
     end
-  | (ED_global i, ET_glob gt) =>
+  | (ED_global (Mk_globalidx i), ET_glob gt) =>
     (i < List.length c.(tc_global)) &&
     match List.nth_error c.(tc_global) i with
     | None => false
@@ -396,7 +399,7 @@ Definition module_typing (m : module) (impts : list extern_t) (expts : list exte
     tc_func_t := List.app ifts fts;
     tc_global := List.app igs gts;
     tc_table := List.app its (List.map (fun t => t.(t_type)) ts);
-    tc_memory := List.app ims ms;
+    tc_memory := List.map (fun '(Mk_mem_type lim) => lim) (List.app ims ms); (* TODO: should use `mem_type`s *)
     tc_local := nil;
     tc_label := nil;
     tc_return := None;
@@ -428,25 +431,25 @@ Inductive external_typing : store_record -> v_ext -> extern_t -> Prop :=
   i < List.length s.(s_funcs) ->
   List.nth_error s.(s_funcs) i = Some cl ->
   tf = operations.cl_type cl ->
-  external_typing s (ED_func i) (ET_func tf)
+  external_typing s (ED_func (Mk_funcidx i)) (ET_func tf)
 | ETY_tab :
   forall (s : store_record) (i : nat) (ti : tableinst) lim,
   i < List.length s.(s_tables) ->
   List.nth_error s.(s_tables) i = Some ti ->
   typing.tab_typing ti lim ->
-  external_typing s (ED_table i) (ET_tab {| tt_limits := lim; tt_elem_type := ELT_funcref |})
+  external_typing s (ED_table (Mk_tableidx i)) (ET_tab {| tt_limits := lim; tt_elem_type := ELT_funcref |})
 | ETY_mem :
   forall (s : store_record) (i : nat) (m : memory) (mt : mem_type),
   i < List.length s.(s_mems) ->
   List.nth_error s.(s_mems) i = Some m ->
   typing.mem_typing m mt ->
-  external_typing s (ED_mem i) (ET_mem mt)
+  external_typing s (ED_mem (Mk_memidx i)) (ET_mem mt)
 | ETY_glob :
   forall (s : store_record) (i : nat) (g : global) (gt : global_type),
   i < List.length s.(s_globals) ->
   List.nth_error s.(s_globals) i = Some g ->
   typing.global_agree g gt ->
-  external_typing s (ED_global i) (ET_glob gt).
+  external_typing s (ED_global (Mk_globalidx i)) (ET_glob gt).
 
 Definition instantiate_globals inst s' m g_inits : Prop :=
   List.Forall2 (fun g v => opsem.reduce_trans inst (s', nil, operations.to_e_list g.(mg_init) ) (s', nil, cons (Basic (EConst v)) nil)) m.(mod_globals) g_inits.
@@ -471,7 +474,7 @@ Definition nat_of_int (i : i32) : nat :=
 Definition check_bounds_elem (inst : instance) (s : store_record) (m : module) (e_offs : seq i32) : bool :=
   seq.all2
     (fun e_off e =>
-      match List.nth_error inst.(i_tab) e.(elem_table) with
+      match List.nth_error inst.(i_tab) (match e.(elem_table) with Mk_tableidx i => i end) with
       | None => false
       | Some i =>
         match List.nth_error s.(s_tables) i with
@@ -489,7 +492,7 @@ Definition mem_length (m : memory) :=
 Definition check_bounds_data (inst : instance) (s : store_record) (m : module) (d_offs : seq i32) : bool :=
   seq.all2
     (fun d_off d =>
-      match List.nth_error inst.(i_memory) d.(dt_data) with
+      match List.nth_error inst.(i_memory) (match d.(dt_data) with Mk_memidx i => i end) with
       | None => false
       | Some i =>
         match List.nth_error s.(s_mems) i with
@@ -504,7 +507,8 @@ Definition check_bounds_data (inst : instance) (s : store_record) (m : module) (
 Definition check_start m inst start : bool :=
   let start' :=
     operations.option_bind
-    (fun i_s => match List.nth_error inst.(i_funcs) i_s.(start_func) with None => None | Some f => Some f end)
+    (fun i_s =>
+      List.nth_error inst.(i_funcs) (match i_s.(start_func) with Mk_funcidx i => i end))
     m.(mod_start) in
   start' == start.
 
@@ -592,28 +596,28 @@ Definition module_imports_typer (tfs : list function_type) (imps : list module_i
 
 Definition module_export_typer (c : t_context) (exp : module_export_desc) : option extern_t :=
   match exp with
-  | ED_func i =>
+  | ED_func (Mk_funcidx i) =>
     if i < List.length c.(tc_func_t) then
       match List.nth_error c.(tc_func_t) i with
       | None => None
       | Some ft => Some (ET_func ft)
       end
     else None
-  | ED_table i =>
+  | ED_table (Mk_tableidx i) =>
     if i < List.length c.(tc_table) then
       match List.nth_error c.(tc_table) i with
       | None => None
       | Some t_t => Some (ET_tab t_t)
       end
     else None
-  | ED_mem i =>
+  | ED_mem (Mk_memidx i) =>
     if i < List.length c.(tc_memory) then
       match List.nth_error c.(tc_memory) i with
       | None => None
-      | Some m => Some (ET_mem m)
+      | Some lim => Some (ET_mem (Mk_mem_type lim))
       end
     else None
-  | ED_global i =>
+  | ED_global (Mk_globalidx i) =>
     if i < List.length c.(tc_global) then
       match List.nth_error c.(tc_global) i with
       | None => None
@@ -658,14 +662,14 @@ Definition module_glob_type_checker (c : t_context) (mg : module_glob) : bool :=
   type_checker.b_e_type_checker c es (Tf nil (cons tg.(tg_t) nil)).
 
 Definition module_elem_type_checker (c : t_context) (e : module_element) : bool :=
-  let '{| elem_table := t; elem_offset := es; elem_init := is_ |} := e in
+  let '{| elem_table := Mk_tableidx t; elem_offset := es; elem_init := is_ |} := e in
   const_exprs c es &&
   type_checker.b_e_type_checker c es (Tf nil (cons T_i32 nil)) &&
   (t < List.length c.(tc_table)) &&
-  seq.all (fun i => i < List.length c.(tc_func_t)) is_.
+  seq.all (fun '(Mk_funcidx i) => i < List.length c.(tc_func_t)) is_.
 
 Definition module_data_type_checker (c : t_context) (d : module_data) : bool :=
-  let '{| dt_data := d; dt_offset := es; dt_init := bs |} := d in
+  let '{| dt_data := Mk_memidx d; dt_offset := es; dt_init := bs |} := d in
   const_exprs c es &&
   type_checker.b_e_type_checker c es (Tf nil (cons T_i32 nil)) &&
   (d < List.length c.(tc_memory)).
@@ -693,8 +697,25 @@ Definition module_type_checker (m : module) : option ((list extern_t) * (list ex
     let ims := ext_t_mems impts in
     let igs := ext_t_globs impts in
     let gts := gather_m_g_types gs in
-    let c := {| tc_types_t := tfs; tc_func_t := List.app ifts fts; tc_global := List.app igs gts; tc_table := List.app its (List.map (fun t => t.(t_type)) ts); tc_memory := List.app ims ms; tc_local := nil; tc_label := nil; tc_return := None |} in
-    let c' := {| tc_types_t := nil; tc_func_t := nil; tc_global := igs; tc_table := nil; tc_memory := nil; tc_local := nil; tc_label := nil; tc_return := None |} in
+    let c := {|
+      tc_types_t := tfs;
+      tc_func_t := List.app ifts fts;
+      tc_global := List.app igs gts;
+      tc_table := List.app its (List.map (fun t => t.(t_type)) ts);
+      tc_memory := List.map (fun '(Mk_mem_type lim) => lim) (List.app ims ms);
+      tc_local := nil;
+      tc_label := nil;
+      tc_return := None |} in
+    let c' := {|
+      tc_types_t := nil;
+      tc_func_t := nil;
+      tc_global := igs;
+      tc_table := nil;
+      tc_memory := nil;
+      tc_local := nil;
+      tc_label := nil;
+      tc_return := None
+    |} in
     if seq.all (module_func_type_checker c) fs &&
        seq.all module_tab_type_checker ts &&
        seq.all module_mem_type_checker ms &&
@@ -712,26 +733,26 @@ Definition module_type_checker (m : module) : option ((list extern_t) * (list ex
 
 Definition external_type_checker (s : store_record) (v : v_ext) (e : extern_t) : bool :=
   match (v, e) with
-  | (ED_func i, ET_func tf) =>
+  | (ED_func (Mk_funcidx i), ET_func tf) =>
     (i < List.length s.(s_funcs)) &&
     match List.nth_error s.(s_funcs) i with
     | None => false
     | Some cl => tf == operations.cl_type cl
     end
-  | (ED_table i, ET_tab tf) =>
+  | (ED_table (Mk_tableidx i), ET_tab tf) =>
     let '{| tt_limits := lim; tt_elem_type := elem_type_tt |} := tf in
     (i < List.length s.(s_tables)) &&
     match List.nth_error s.(s_tables) i with
     | None => false
     | Some ti => typing.tab_typing ti lim
     end
-  | (ED_mem i, ET_mem mt) =>
+  | (ED_mem (Mk_memidx i), ET_mem mt) =>
     (i < List.length s.(s_mems)) &&
     match List.nth_error s.(s_mems) i with
     | None => false
     | Some m => typing.mem_typing m mt
     end
-  | (ED_global i, ET_glob gt) =>
+  | (ED_global (Mk_globalidx i), ET_glob gt) =>
     (i < List.length s.(s_globals)) &&
     match List.nth_error s.(s_globals) i with
     | None => false
@@ -739,8 +760,6 @@ Definition external_type_checker (s : store_record) (v : v_ext) (e : extern_t) :
     end
   | (_, _) => false
   end.
-
-Require interpreter.
 
 Definition interp_get_v (s : store_record) (inst : instance) (b_es : list basic_instruction) : option value (* TODO: isa mismatch *) :=
   match interpreter.run_v 2 0 inst (s, nil, operations.to_e_list b_es) with
@@ -769,7 +788,7 @@ Definition interp_instantiate (s : store_record) (m : module) (v_imps : list v_e
           i_funcs := nil;
           i_tab := nil;
           i_memory := nil;
-          i_globs := ext_globs v_imps;
+          i_globs := List.map (fun '(Mk_globalidx i) => i) (ext_globs v_imps);
         |} in
         those (map (fun g => interp_get_v s c g.(mg_init)) m.(mod_globals)) in
       match g_inits_opt with
@@ -786,7 +805,7 @@ Definition interp_instantiate (s : store_record) (m : module) (v_imps : list v_e
           | Some d_offs =>
             if check_bounds_elem inst s m e_offs &&
                check_bounds_data inst s m d_offs then
-              let start : option nat := operations.option_bind (fun i_s => List.nth_error inst.(i_funcs) i_s.(start_func)) m.(mod_start) in
+              let start : option nat := operations.option_bind (fun i_s => List.nth_error inst.(i_funcs) (match i_s.(start_func) with Mk_funcidx i => i end)) m.(mod_start) in
               let s'' := init_tabs s' inst (map nat_of_int e_offs) m.(mod_elem) in
               let s_end := init_mems s' inst (map nat_of_int d_offs) m.(mod_data) in
               Some ((s_end, inst, v_exps), start)
